refactor: Rename [program] into [impure], and document the library
This may probably be a very controversial change. This commit rename
the [program] monad into [impure], talks about impure computations
rather than programs with effects and impure primitives rather than
effects.

One reason behind this choice is to avoid any confusion with the
Program framework of Coq. The main reason, however, is that our monad
is more limited compare to algebraic effects, as they are described in
the literature.

Besides, we provide more documentation about the FreeSpec.Core.Impure
library.

core/examples/airlock.v
@@ -33,17 +33,17 @@ Inductive DOORS : interface :=
 
 Generalizable All Variables.
 
-Definition is_open `{ix :| DOORS} (d : door) : program ix bool :=
+Definition is_open `{ix :| DOORS} (d : door) : impure ix bool :=
   request (IsOpen d).
 
-Definition toggle `{ix :| DOORS} (d : door) : program ix unit :=
+Definition toggle `{ix :| DOORS} (d : door) : impure ix unit :=
   request (Toggle d).
 
-Definition open_door `{ix :| DOORS} (d : door) : program ix unit :=
+Definition open_door `{ix :| DOORS} (d : door) : impure ix unit :=
   var open ← is_open d in
   when (negb open) (toggle d).
 
-Definition close_door `{ix :| DOORS} (d : door) : program ix unit :=
+Definition close_door `{ix :| DOORS} (d : door) : impure ix unit :=
   var open ← is_open d in
   when open (toggle d).
 
@@ -53,10 +53,10 @@ Inductive CONTROLLER : interface :=
 | Tick : CONTROLLER unit
 | RequestOpen (d : door) : CONTROLLER unit.
 
-Definition tick `{ix :| CONTROLLER} : program ix unit :=
+Definition tick `{ix :| CONTROLLER} : impure ix unit :=
   request Tick.
 
-Definition request_open `{ix :| CONTROLLER} (d : door) : program ix unit :=
+Definition request_open `{ix :| CONTROLLER} (d : door) : impure ix unit :=
   request (RequestOpen d).
 
 Definition co (d : door) : door :=
@@ -112,34 +112,34 @@ Qed.
 
 Opaque tog.
 
-Definition step (a : Type) (ω : Ω) (e : DOORS a) (x : a) :=
+Definition step (ω : Ω) (a : Type) (e : DOORS a) (x : a) :=
   match e with
   | Toggle d => tog d ω
   | _ => ω
   end.
 
-Inductive req : forall (a : Type), Ω -> DOORS a -> Prop :=
+Inductive req : Ω -> forall (a : Type), DOORS a -> Prop :=
 (** Given the door [d] of o system [ω], it is always possible to ask for the
     state of [d]. *)
 | req_is_open (d : door) (ω : Ω)
-  : req bool ω (IsOpen d)
+  : req ω bool (IsOpen d)
 
 (** Given the door [d] of o system [ω], if [d] is closed, then the second door
     [co d] has to be closed to for a request to toggle [d] to be valid. *)
 | req_toggle (d : door) (ω : Ω) (H : sel d ω = false -> sel (co d) ω = false)
-  : req unit ω (Toggle d).
+  : req ω unit (Toggle d).
 
-Inductive prom: forall (a : Type), Ω -> DOORS a -> a -> Prop :=
+Inductive prom: Ω -> forall (a : Type), DOORS a -> a -> Prop :=
 
 (** When a system in a state [ω] reports the state of the door [d], it shall
     reflect the true state of [d]. *)
 | prom_is_open (d : door) (ω : Ω) (x : bool) (equ : sel d ω = x)
-  : prom bool ω (IsOpen d) x
+  : prom ω bool (IsOpen d) x
 
 (** There is no particular promises on the result [x] of a request for [ω] to
     close the door [d]. *)
 | prom_toggle (d : door) (ω : Ω) (x : unit)
-  : prom unit ω (Toggle d) x.
+  : prom ω unit (Toggle d) x.
 
 Definition doors_specs : specs DOORS Ω := Build_specs _ _ step req prom.
 
@@ -147,11 +147,11 @@ From Prelude Require Import Tactics.
 
 (** Closing a door [d] in any system [ω] is always a trustworthy operation. *)
 Lemma close_door_trustworthy (ω : Ω) (d : door)
-  : trustworthy_program doors_specs ω (close_door d).
+  : trustworthy_impure doors_specs ω (close_door d).
 
 Proof.
   (* We use the [prove_program] tactics to erease the program monad *)
-  prove_program; cbn; repeat constructor; subst.
+  prove_impure; cbn; repeat constructor; subst.
   (* This leaves us with one goal to prove:
 
        [sel d ω = false -> sel (co d) ω = false]
@@ -164,15 +164,15 @@ Proof.
 Qed.
 
 Lemma open_door_trustworthy (ω : Ω) (d : door) (safe : sel (co d) ω = false)
-  : trustworthy_program doors_specs ω (open_door d).
+  : trustworthy_impure doors_specs ω (open_door d).
 
 Proof.
-  prove_program; cbn; repeat constructor; subst.
+  prove_impure; cbn; repeat constructor; subst.
   inversion Hpost; ssubst.
   now rewrite safe.
 Qed.
 
-Definition safe_open_door {ix} `{ix :| DOORS} (d : door) : program ix unit :=
+Definition safe_open_door {ix} `{ix :| DOORS} (d : door) : impure ix unit :=
   do close_door (co d);
      open_door d.
 
@@ -196,10 +196,10 @@ Qed.
 #[local] Opaque open_door.
 
 Lemma safe_door_trustworthy (ω : Ω) (d : door)
-  : trustworthy_program doors_specs ω (safe_open_door d).
+  : trustworthy_impure doors_specs ω (safe_open_door d).
 
 Proof.
-  prove_program; cbn; repeat constructor; subst.
+  prove_impure; cbn; repeat constructor; subst.
   apply close_door_trustworthy.
   apply close_door_run in Hrun.
   apply open_door_trustworthy.
