core/theories/Core/Specs.v
@@ -20,7 +20,7 @@
 
 From Coq Require Import Setoid Morphisms.
 From Prelude Require Import Tactics Equality.
-From FreeSpec.Core Require Export Program.
+From FreeSpec.Core Require Export Impure.
 
 #[local]
 Open Scope prelude_scope.
@@ -76,37 +76,36 @@ Bind Scope specs_scope with specs.
 
 (** * Reasoning with Specifications
 
-    ** Program Trustworthiness
+    ** Impure Computation Trustworthiness
 
-    A program [p] is said trustworthy wrt. a specification [c] in accordance to
-    a witness [ω] when it only uses effects of [i] which satisfies [c]
-    requirements. *)
+    An impure computation [p] is said trustworthy wrt. a specification [c] in
+    accordance to a witness [ω] when it only uses primitives of [i] which
+    satisfies [c] requirements. *)
 
-Inductive trustworthy_program {i a Ω} (c : specs i Ω) (ω : Ω) : program i a -> Prop :=
+Inductive trustworthy_impure {i a Ω} (c : specs i Ω) (ω : Ω) : impure i a -> Prop :=
 
-(**  - Given a term [x], the program [local x] is always
-      trustworthy wrt. [c] in accordance to [ω], since it does not use any
-      effects. *)
+(** - Given a term [x], the computation [local x] is always trustworthy wrt. [c]
+      in accordance to [ω], since it does not use any primitives. *)
 | trustworthy_local (x : a)
-  : trustworthy_program c ω (local x)
+  : trustworthy_impure c ω (local x)
 
-(** - Given an effect [e] and a continuation [f], if
+(** - Given a primitive [e] and a continuation [f], if
 
       - [e] satisfies [c] requirements
-      - [f] programs are trustworthy wrt. [c] in accordance to [ω'], where [ω'] is
-        the witness after [e] interpretation
+      - [f] computations are trustworthy wrt. [c] in accordance to [ω'], where
+        [ω'] is the witness after [e] interpretation
 
-      then the program [request_then e f] is trustworthy wrt. [c] in accordance to
-      [ω]. *)
+      then the impure computation [request_then e f] is trustworthy wrt. [c] in
+      accordance to [ω]. *)
 | trustworthy_request {b}
-    (e : i b) (req : requirements c ω e) (f : b -> program i a)
+    (e : i b) (req : requirements c ω e) (f : b -> impure i a)
     (prom : forall (x : b),
-        promises c ω e x -> trustworthy_program c (witness_update c ω e x) (f x))
-  : trustworthy_program c ω (request_then e f).
+        promises c ω e x -> trustworthy_impure c (witness_update c ω e x) (f x))
+  : trustworthy_impure c ω (request_then e f).
 
 #[program]
-Instance trustworthy_program_Proper {i Ω} (a : Type) (c : specs i Ω) (ω : Ω)
-  : Proper ('equal ==> Basics.impl) (trustworthy_program (a:=a) c ω).
+Instance trustworthy_impure_Proper {i Ω} (a : Type) (c : specs i Ω) (ω : Ω)
+  : Proper ('equal ==> Basics.impl) (trustworthy_impure (a:=a) c ω).
 
 Next Obligation.
   add_morphism_tactic.
@@ -125,7 +124,7 @@ Next Obligation.
 Qed.
 
 Inductive trustworthy_run {i a Ω} (c : specs i Ω)
-  : program i a -> Ω -> Ω -> a -> Prop :=
+  : impure i a -> Ω -> Ω -> a -> Prop :=
 
 (** Given a term [x], and an initial witness [ω], then a trustworthy run of
     [local x] produces a result [x] and a witness state [ω]. *)
@@ -133,29 +132,29 @@ Inductive trustworthy_run {i a Ω} (c : specs i Ω)
     (x : a) (ω : Ω)
   : trustworthy_run c (local x) ω ω x
 
-(** Given an initial witness [ω], an effect [e] which satisfies [c]
+(** Given an initial witness [ω], a primitive [e] which satisfies [c]
     requirements, and a continuation [f], a result [x] for [e] which satisfies
     [c] promises, if we can show that there is a trustworthy run of [f x]
     which produces a term [y] and a witness [ω'], then there is a trustworthy
     run of [request_then e f] which produces a result [y] and a witness [ω']. *)
 | run_request {b}
     (ω : Ω)
-    (e : i b) (req : requirements c ω e) (f : b -> program i a)
+    (e : i b) (req : requirements c ω e) (f : b -> impure i a)
     (x : b) (prom : promises c ω e x)
     (ω' : Ω) (y : a) (rec : trustworthy_run c (f x) (witness_update c ω e x) ω' y)
   : trustworthy_run c (request_then e f) ω ω' y.
 
-(** Given a specification [c] and a witness [ω] a program of effects [p] and a
+(** Given a specification [c] and a witness [ω] an impure computation [p] and a
     continuation [f] if [p] is a trustworthy program wrt. [c] in accordance to
     [ω] and for all result [x] and witness [ω'] produces by [p], [f x] is
     trustworthy then [local p f] is trustworthy. *)
-Lemma lm_trustworthy_bind_trustworthy_run {i a b Ω}
+Lemma trustworthy_bind_trustworthy_run {i a b Ω}
   (c : specs i Ω) (ω : Ω)
-  (p : program i a) (f : a -> program i b)
-  (trust : trustworthy_program c ω p)
+  (p : impure i a) (f : a -> impure i b)
+  (trust : trustworthy_impure c ω p)
   (run : forall (x : a) (ω' : Ω),
-      trustworthy_run c p ω ω' x -> trustworthy_program c ω' (f x))
-  : trustworthy_program c ω (program_bind p f).
+      trustworthy_run c p ω ω' x -> trustworthy_impure c ω' (f x))
+  : trustworthy_impure c ω (impure_bind p f).
 
 Proof.
   revert ω trust run.
@@ -173,7 +172,7 @@ Proof.
        econstructor; eauto.
 Qed.
 
-Hint Resolve lm_trustworthy_bind_trustworthy_run : freespec_scope.
+Hint Resolve trustworthy_bind_trustworthy_run : freespec_scope.
 
 (** ** Semantics Compliance *)
 
@@ -194,7 +193,7 @@ CoInductive compliant_semantics {i Ω} (c : specs i Ω) : Ω -> semantics i -> P
 (** … then [sem] complies to [c] in accordance to [ω] *)
   : compliant_semantics c ω sem.
 
-Lemma lm_compliant_semantics_requirement_promises {i Ω a} (c : specs i Ω) (ω : Ω)
+Lemma compliant_semantics_requirement_promises {i Ω a} (c : specs i Ω) (ω : Ω)
   (e : i a) (req : requirements c ω e)
   (sem : semantics i) (comp : compliant_semantics c ω sem)
   : promises c ω e (eval_effect sem e).
@@ -204,9 +203,9 @@ Proof.
   now apply prom.
 Qed.
 
-Hint Resolve lm_compliant_semantics_requirement_promises : freespec.
+Hint Resolve compliant_semantics_requirement_promises : freespec.
 
-Lemma lm_compliant_semantics_requirement_compliant {i Ω a} (c : specs i Ω) (ω : Ω)
+Lemma compliant_semantics_requirement_compliant {i Ω a} (c : specs i Ω) (ω : Ω)
   (e : i a) (req : requirements c ω e)
   (sem : semantics i) (comp : compliant_semantics c ω sem)
   : compliant_semantics c (witness_update c ω e (eval_effect sem e)) (exec_effect sem e).
@@ -216,9 +215,9 @@ Proof.
   now apply next.
 Qed.
 
-Hint Resolve lm_compliant_semantics_requirement_compliant : freespec.
+Hint Resolve compliant_semantics_requirement_compliant : freespec.
 
-Lemma lm_compliant_semantics_exec_effect_equ {i Ω a} (c : specs i Ω) (ω : Ω)
+Lemma compliant_semantics_exec_effect_equ {i Ω a} (c : specs i Ω) (ω : Ω)
   (sem sem' : semantics i) (equ : sem == sem')
   (e : i a)
   : exec_effect sem e == exec_effect sem' e.
@@ -228,7 +227,7 @@ Proof.
   now inversion step_equiv; ssubst.
 Qed.
 
-Hint Resolve lm_compliant_semantics_exec_effect_equ : freespec.
+Hint Resolve compliant_semantics_exec_effect_equ : freespec.
 
 #[program]
 Instance compliant_semantics_Proper {i Ω} (c : specs i Ω) (ω : Ω)
@@ -249,7 +248,7 @@ Next Obligation.
        now apply next.
 Qed.
 
-Lemma lm_no_specs_compliant_semantics {i}
+Lemma no_specs_compliant_semantics {i}
   (sem : semantics i) (ϵ : unit)
   : compliant_semantics (no_specs i) ϵ sem.
 
@@ -262,9 +261,9 @@ Proof.
     apply no_specs_compliant_semantics.
 Qed.
 
-Hint Resolve lm_no_specs_compliant_semantics : freespec.
+Hint Resolve no_specs_compliant_semantics : freespec.
 
-Lemma lm_compliant_semantics_semplus {i j Ωi Ωj}
+Lemma compliant_semantics_semplus {i j Ωi Ωj}
   (semi : semantics i) (semj : semantics j)
   (ci : specs i Ωi) (ωi : Ωi) (compi : compliant_semantics ci ωi semi)
   (cj : specs j Ωj) (ωj : Ωj) (compj : compliant_semantics cj ωj semj)
@@ -272,18 +271,18 @@ Lemma lm_compliant_semantics_semplus {i j Ωi Ωj}
 
 Proof.
   revert ωi ωj semi semj compi compj.
-  cofix lm_compliant_semantics_semplus; intros ωi ωj semi semj compi compj.
+  cofix compliant_semantics_semplus; intros ωi ωj semi semj compi compj.
   constructor; intros a e req.
   + destruct e; [ inversion compi | inversion compj ]; ssubst; now apply prom.
   + destruct e; [ inversion compi | inversion compj ]; ssubst;
-      apply lm_compliant_semantics_semplus;
+      apply compliant_semantics_semplus;
       auto;
       now apply next.
 Qed.
 
-Hint Resolve lm_compliant_semantics_semplus : freespec.
+Hint Resolve compliant_semantics_semplus : freespec.
 
-Lemma lm_compliant_semantics_semplus_no_specs {i j Ω}
+Lemma compliant_semantics_semplus_no_specs {i j Ω}
   (ci : specs i Ω) (ω : Ω) (semi : semantics i) (comp : compliant_semantics ci ω semi)
   (semj : semantics j) (ϵ : unit)
   : compliant_semantics (ci ⊙ no_specs j) (ω, ϵ) (semi ⊗ semj).
@@ -293,19 +292,19 @@ Proof.
 Qed.
 
 #[local]
-Fixpoint witness_program_aux {i Ω a}
-  (sem : semantics i) (p : program i a) (c : specs i Ω) (ω : Ω) : interp_out i a * Ω :=
+Fixpoint witness_impure_aux {i Ω a}
+  (sem : semantics i) (p : impure i a) (c : specs i Ω) (ω : Ω) : interp_out i a * Ω :=
   match p with
   | local x => (mk_out x sem, ω)
   | request_then e f =>
     let out := run_effect sem e in
     let res := interp_result out in
-    witness_program_aux (interp_next out) (f res) c (witness_update c ω e res)
+    witness_impure_aux (interp_next out) (f res) c (witness_update c ω e res)
   end.
 
-Lemma fst_witness_program_aux_run_program {i Ω a}
-  (sem : semantics i) (p : program i a) (c : specs i Ω) (ω : Ω)
-  : fst (witness_program_aux sem p c ω) = run_program sem p.
+Lemma fst_witness_impure_aux_run_impure {i Ω a}
+  (sem : semantics i) (p : impure i a) (c : specs i Ω) (ω : Ω)
+  : fst (witness_impure_aux sem p c ω) = run_impure sem p.
 
 Proof.
   revert sem ω.
@@ -314,27 +313,27 @@ Proof.
   + apply H.
 Qed.
 
-Hint Rewrite @fst_witness_program_aux_run_program : freespec.
+Hint Rewrite @fst_witness_impure_aux_run_impure : freespec.
 
-Definition witness_program {i Ω a}
-  (sem : semantics i) (p : program i a) (c : specs i Ω) (ω : Ω) : Ω :=
-  snd (witness_program_aux sem p c ω).
+Definition witness_impure {i Ω a}
+  (sem : semantics i) (p : impure i a) (c : specs i Ω) (ω : Ω) : Ω :=
+  snd (witness_impure_aux sem p c ω).
 
-Lemma witness_progran_request_then_equ {i Ω a b} (c : specs i Ω) (ω : Ω)
-  (sem : semantics i) (e : i a) (f : a -> program i b)
-  : witness_program sem (request_then e f) c ω
-    = witness_program (exec_effect sem e)
-                      (f (eval_effect sem e))
-                      c
-                      (witness_update c ω e (eval_effect sem e)).
+Lemma witness_impure_request_then_equ {i Ω a b} (c : specs i Ω) (ω : Ω)
+  (sem : semantics i) (e : i a) (f : a -> impure i b)
+  : witness_impure sem (request_then e f) c ω
+    = witness_impure (exec_effect sem e)
+                     (f (eval_effect sem e))
+                     c
+                     (witness_update c ω e (eval_effect sem e)).
 Proof eq_refl.
 
-Hint Rewrite @witness_progran_request_then_equ : freespec.
+Hint Rewrite @witness_impure_request_then_equ : freespec.
 
-Lemma lm_trustworthy_program_compliant_specs {i Ω a} (c : specs i Ω) (ω : Ω)
-  (p : program i a) (trust : trustworthy_program c ω p)
+Lemma trustworthy_impure_compliant_specs {i Ω a} (c : specs i Ω) (ω : Ω)
+  (p : impure i a) (trust : trustworthy_impure c ω p)
   (sem : semantics i) (comp : compliant_semantics c ω sem)
-  : compliant_semantics c (witness_program sem p c ω) (exec_program sem p).
+  : compliant_semantics c (witness_impure sem p c ω) (exec_impure sem p).
 
 Proof.
   revert trust sem comp. revert ω.
@@ -345,7 +344,7 @@ Proof.
     apply H; auto with freespec.
 Qed.
 
-Hint Resolve lm_trustworthy_program_compliant_specs : freespec.
+Hint Resolve trustworthy_impure_compliant_specs : freespec.
 
 (** ** Component Correctness *)
 
@@ -363,10 +362,10 @@ Hint Resolve lm_trustworthy_program_compliant_specs : freespec.
 >>
 
     We say [c] is correct wrt. [speci] (a specification for [i]) and [specj] (a
-    specification for [i]) iff given effects which satisfy the requirements of
+    specification for [i]) iff given primitives which satisfy the requirements of
     [speci], [c] will
 
-    - use trustworthy program wrt. [specj]
+    - use trustworthy impure computations wrt. [specj]
     - compute results which satisfy [speci] promises, assuming it can rely on a
       semantics of [j] which complies with [specj]
 
@@ -384,18 +383,18 @@ Definition correct_component {i j Ωi Ωj s}
   forall (ωi : Ωi) (st : s) (ωj : Ωj) (init : pred ωi st ωj)
     (sem : semantics j) (comp : compliant_semantics specj ωj sem)
     (a : Type) (e : i a) (req : requirements speci ωi e),
-    trustworthy_program specj ωj (c a e st)
-    /\ promises speci ωi e (fst (eval_program sem (c a e st)))
-    /\ pred (witness_update speci ωi e (fst (eval_program sem (c a e st))))
-            (snd (eval_program sem (c a e st)))
-            (witness_program sem (c a e st) specj ωj).
+    trustworthy_impure specj ωj (c a e st)
+    /\ promises speci ωi e (fst (eval_impure sem (c a e st)))
+    /\ pred (witness_update speci ωi e (fst (eval_impure sem (c a e st))))
+            (snd (eval_impure sem (c a e st)))
+            (witness_impure sem (c a e st) specj ωj).
 
 (** Once we have proven [c] is correct wrt. to [speci] and [specj] with [pred]
     acting as an invariant throughout [c] life, we show we can derive a
     semantics from [c] with an initial state [st] which complies to [speci] in
     accordance to [ωi] if we use a semantics of [j] which complies to [specj] in
     accordance to [ωj], where [pred ωi st ωj] is satisfied. *)
-Lemma lm_correct_component_derives_compliant_semantics {i j Ωi Ωj s}
+Lemma correct_component_derives_compliant_semantics {i j Ωi Ωj s}
   (c : component i j s) (speci : specs i Ωi) (specj : specs j Ωj)
   (pred : Ωi -> s -> Ωj -> Prop)
   (correct : correct_component c speci specj pred)
@@ -406,17 +405,17 @@ Lemma lm_correct_component_derives_compliant_semantics {i j Ωi Ωj s}
 Proof.
   revert inv sem comp.
   revert ωi st ωj.
-  cofix lm_correct_component_derives_compliant_semantics.
+  cofix correct_component_derives_compliant_semantics.
   intros ωi st ωj inv sem comp.
   unfold correct_component in correct.
   specialize (correct ωi st ωj inv sem comp).
   constructor; intros a e req; specialize (correct a e req);
     destruct correct as [trust [pr inv']].
   + apply pr.
-  + eapply lm_correct_component_derives_compliant_semantics.
+  + eapply correct_component_derives_compliant_semantics.
     ++ apply inv'.
-    ++ fold (exec_program sem (c a e st)).
-       apply lm_trustworthy_program_compliant_specs; [| exact comp ].
+    ++ fold (exec_impure sem (c a e st)).
+       apply trustworthy_impure_compliant_specs; [| exact comp ].
        apply trust.
 Qed.
 
@@ -435,24 +434,24 @@ Ltac destruct_if_when :=
   | _ => idtac
   end.
 
-Ltac prove_program :=
+Ltac prove_impure :=
   repeat (cbn; destruct_if_when);
   lazymatch goal with
   (* 1st case: nested bind:
        rewrite ((p >>= f) >>= g) into p >>= (λ x, f x >>= g) *)
-  | |- trustworthy_program ?c ?w (program_bind (program_bind ?p ?f) ?g) =>
-    rewrite (lm_program_bind_assoc p f g); prove_program
+  | |- trustworthy_impure ?c ?w (impure_bind (impure_bind ?p ?f) ?g) =>
+    rewrite (impure_bind_assoc p f g); prove_impure
   (* 2nd case: bind opaque program:
        rely on the correct_run abstraction *)
-  | |- trustworthy_program ?c ?w (program_bind ?p ?f) =>
+  | |- trustworthy_impure ?c ?w (impure_bind ?p ?f) =>
     let x := fresh "x" in
     let w := fresh "w" in
     let Hrun := fresh "Hrun" in
-    apply lm_trustworthy_bind_trustworthy_run; [| intros x w Hrun;
-                                                  prove_program ]
+    apply trustworthy_bind_trustworthy_run; [| intros x w Hrun;
+                                                  prove_impure ]
   (* 3rd case: request constructor
       generate a gool to prove the effect satisfies the precondition *)
-  | |- trustworthy_program ?c ?w (request_then ?e ?f) =>
+  | |- trustworthy_impure ?c ?w (request_then ?e ?f) =>
     let Hpre := fresh "Hpre" in
     assert (Hpre: requirements c w e); [| constructor; [apply Hpre |];
                                           let sig := fresh "sig" in
@@ -460,10 +459,10 @@ Ltac prove_program :=
                                           let res := fresh "res" in
                                           let Hpost := fresh "Hpost" in
                                           intros res Hpost;
-                                          prove_program ]
+                                          prove_impure ]
   (* 4st case: pure constructor
        conclude *)
-  | |- trustworthy_program ?c ?w (local ?x) => constructor
-  | |- trustworthy_program ?c ?w (program_pure ?x) => constructor
+  | |- trustworthy_impure ?c ?w (local ?x) => constructor
+  | |- trustworthy_impure ?c ?w (impure_pure ?x) => constructor
   | _ => fail "Unexpected goal: prove_program allows for proving program correctness"
   end.
