core/theories/Core/Impure.v
@@ -1,0 +1,958 @@
+(* FreeSpec
+ * Copyright (C) 2018–2019 ANSSI
+ *
+ * Contributors:
+ * 2018–2019 Thomas Letan <thomas.letan@ssi.gouv.fr>
+ *
+ * This impure is free software: you can redistribute it and/or modify
+ * it under the terms of the GNU General Public License as published by
+ * the Free Software Foundation, either version 3 of the License, or
+ * (at your option) any later version.
+ *
+ * This impure is distributed in the hope that it will be useful,
+ * but WITHOUT ANY WARRANTY; without even the implied warranty of
+ * MERCHANTABILITY or FITNESS FOR A PARTICULAR PURPOSE.  See the
+ * GNU General Public License for more details.
+ *
+ * You should have received a copy of the GNU General Public License
+ * along with this program. If not, see <http://www.gnu.org/licenses/>.
+ *)
+
+(** In this library, we provide all the necessary concepts to model interacting
+    components using Coq.  We do that by means of a variant of the Free monad
+    introduced by the Haskell ~operational~ package, and originally called the
+    Program monad thereafter.  The Program monad is parameterized by a type
+    which describes the interfaces its monadic computations can use, where an
+    interface describes a set of functions carried out by an outer environment
+    expected to produce a result.  In other words, using the ~operational~
+    Program monad, we model impurity.
+
+    To avoid ambiguity with the Program framework of Coq, we rename the Program
+    monad the [impure] monad, and we call “impure computations” the monadic
+    computations which happens within the [impure] monad.  We call “primitives”
+    the impure functions provided by a given interface.
+
+    The key idea behind FreeSpec is to model components as functions which maps
+    primitives of the interface it exposes to impure computations parameterized
+    by the interfaces it uses. *)
+
+From Coq.Program Require Import Equality Tactics Basics.
+From Coq Require Import Morphisms.
+From Coq Require Import Relations Setoid Morphisms.
+From Prelude Require Import Equality Control Control.Classes Tactics State.
+From FreeSpec.Core Require Import utils.
+
+#[local]
+Open Scope signature_scope.
+
+#[local]
+Open Scope prelude_scope.
+
+Notation "''equal'" := (@equal _ _) (only parsing).
+
+(** * Interfaces *)
+
+(** Following the definition of the ~operational~ package, interfaces in
+    FreeSpec are parameterized inductive types whose terms purposely describe
+    the primitives the interface provides. *)
+
+Definition interface := Type -> Type.
+
+(** Given [i : interface], a term of type [i α] identifies a primitive of [i]
+    expected to produce a result of type [α].
+
+    The simpler interface is the empty interface, which provides no primitives
+    whatsoever. *)
+
+Inductive iempty : interface := .
+Notation "'<>'" := iempty : type_scope.
+Notation "'⋄'" := iempty : type_scope.
+
+(** To use the [⋄] interface to parameterize the [impure] monad is equivalent to
+    writing pure functions.
+
+    Another example of general-purpose interface we can define is the [STORE s]
+    interface, where [s] is a type, and [STORE s] allows for manipulating a
+    global, mutable variable of type [s] within an impure computation.
+
+<<
+Inductive STORE (s : Type) : interface :=
+| Get : STORE s s
+| Put (x : s) : STORE s unit.
+>>
+
+    According to the definition of [STORE s], an impure computation can use two
+    primitives. The term [Get : STORE s s] describes a primitive expected to
+    produce a result of type [s], that is the current value of the mutable
+    variable.  Terms of the form [Put x : STORE s unit] describe a primitive
+    which does not produce any meaningful result, but is expected to update the
+    current value of the mutable variable.
+
+    The use of the word “expected” to describe the primitive of [STORE s] is
+    voluntary.  The definition of a semantics does not attach any particular
+    semantics to the primitives it describes.  This will come latter, and in
+    fact, one interface may have many legitimate semantics.
+
+    Impure computations are likely to use more than one interface, but the
+    [impure] monad takes only one argument.  We introduce [iplus] (denoted by
+    [<+>] or [⊕]) to compose interfaces together.  An impure computation
+    parameterized by [i ⊕ j] can therefore leverages the privimites of both [i]
+    and [j]. *)
+
+
+Inductive iplus (i j : interface) (a : Type) :=
+| in_left (e : i a) : iplus i j a
+| in_right (e : j a) : iplus i j a.
+
+Arguments in_left [i j a] (e).
+Arguments in_right [i j a] (e).
+
+Infix "<+>" := iplus (at level 50, left associativity) : type_scope.
+Infix "⊕" := iplus (at level 50, left associativity) : type_scope.
+
+(** When defining general-purpose impure computations that we expect to reuse in
+    different context, we want to leave the interface as a parameter, and rather
+    express the constrains in terms of interface availability.  To do that, we
+    introduce the [Provide] typeclass, such that [Provide ix i] implies impure
+    computations parameterized by [ix] can use primitives of [i]. *)
+
+Class Provide (ix i : interface) : Type :=
+  { lift_eff {a : Type} (e : i a) : ix a
+  }.
+
+#[program]
+Instance refl_Provide (i : interface) : Provide i i :=
+  { lift_eff := fun (a : Type) (e : i a) => e
+  }.
+
+#[program]
+Instance iplus_left_Provide (i j : interface) : Provide (i ⊕ j) i :=
+  { lift_eff := @in_left i j
+  }.
+
+#[program]
+Instance iplus_right_Provide (i j : interface) : Provide (i ⊕ j) j :=
+  { lift_eff := @in_right i j
+  }.
+
+(** We introduce a dedicated notation for conveniently declare interface
+    requirements.  Our main source of inspiration is the PureScript row of
+    effects.
+
+    Afterwards, we can write [`{ix :| INTERFACE1, INTERFACE2}] to say that [ix]
+    provides at least [INTERFACE1] and [INTERFACE2] primitives. *)
+
+Notation "ix ':|' i1 ',' i2 ',' .. ',' i3" :=
+  (CCons (Provide ix i1) (CCons (Provide ix i2) .. (CCons (Provide ix i3) CNil) ..))
+    (at level 78, i1, i2, i3 at next level, no associativity)
+  : type_scope.
+
+Notation "ix ':|' i" :=
+  (Provide ix i)
+    (at level 78, i at next level, no associativity)
+  : type_scope.
+
+(* begin hide *)
+#[local]
+Definition provide_notation_test_1 {a}
+  (ix i1 i2 i3 : interface) `{ix :| i1, i2, i3} (p : i2 a) : ix a :=
+  lift_eff p.
+
+#[local]
+Definition provide_notation_test_2 {a}
+  (ix i1 i2 i3 : interface) `{ix :| i1, i2, i3} (p : forall i' `{ix :| i2, i3}, i' a)
+  : ix a :=
+  p ix.
+(* end hide *)
+
+(** * Operational Semantics *)
+
+(** We have already explained interfaces, in FreeSpec, does not attach any
+    particular semantics to their primitives.  Once an interface has been
+    defined, we can provide one (or more) operational semantics to interpret its
+    primitives. *)
+
+(** ** Definition *)
+
+(** An operational [semantics] for the interface [i] is coinductively defined as
+    a function which can be used to interpret any primitive of [i]; it produces
+    an [interp_out] terms. *)
+
+CoInductive semantics (i : interface) : Type :=
+| mk_semantics (f : forall (a : Type), i a -> interp_out i a) : semantics i
+
+(** A term of type [interp_out i a] is therefore the result of the
+    interpretation of a given primitive [i a]. It provides a result for this
+    primitive (of type [a]), and the new semantics to use to interpret the next
+    primitive of [i]. *)
+
+with interp_out (i : interface) : Type -> Type :=
+| mk_out {a} (x : a) (sem : semantics i) : interp_out i a.
+
+(** Thus, a [semantics] does not only compute a result for a primitive, but also
+    provides a new semantics.  This is necessary to model impurity: the same
+    primitive may or may not return the same result when called several
+    times. *)
+
+Arguments mk_semantics [i] (f).
+Arguments mk_out [i a] (x sem).
+
+(** As for interfaces, the simpler [semantics] is the operational semantics for
+    [⋄], the empty interface. *)
+
+Definition semempty : semantics ⋄ :=
+  mk_semantics (fun (a : Type) (e : iempty a) => match e with end).
+
+(** As an example, we provide a semantics for the [STORE s] interface:
+
+<<
+CoFixpoint store {s} (init : s) : semantics (STORE s) :=
+  mk_semantics (fun (a : Type) (e : STORE s a) =>
+                  match e with
+                  | Get => mk_out init (store init)
+                  | Put next => mk_out tt (store next)
+                  end).
+>> *)
+
+(** We provide several helper functions to interpret primitives with
+    semantics. *)
+
+Definition run_effect {i a} (sem : semantics i) (e : i a) : interp_out i a :=
+  match sem with mk_semantics f => f _ e end.
+
+Definition interp_result {i a} (step : interp_out i a) : a :=
+  match step with mk_out x _ => x end.
+
+Definition interp_next {i a} (step : interp_out i a) : semantics i :=
+  match step with mk_out _ sem => sem end.
+
+Definition eval_effect {i a} (sem : semantics i) (e : i a) : a :=
+  interp_result (run_effect sem e).
+
+Definition exec_effect {i a} (sem : semantics i) (e : i a) : semantics i :=
+  interp_next (run_effect sem e).
+
+(** Besides, and similarly to interfaces, operational semantics can and should
+    be composed together.  To that end, we provide the [semplus] operation
+    (denoted by [<+>] or [⊕]). *)
+
+CoFixpoint semplus {i j} (sem_i : semantics i) (sem_j : semantics j)
+  : semantics (i ⊕ j) :=
+  mk_semantics (fun (a : Type) (e : (i ⊕ j) a) =>
+                  match e with
+                  | in_left e =>
+                    let out := run_effect sem_i e in
+                    mk_out (interp_result out) (semplus (interp_next out) sem_j)
+                  | in_right e =>
+                    let out := run_effect sem_j e in
+                    mk_out (interp_result out) (semplus sem_i (interp_next out))
+                  end).
+
+Infix "<x>" := semplus (at level 50, left associativity) : semantics_scope.
+Infix "⊗" := semplus (at level 50, left associativity) : semantics_scope.
+
+Bind Scope semantics_scope with semantics.
+
+(** ** Equivalence *)
+
+(** We say two semantics are equivalent when (1) we they produce equivalent outputs
+    given the same primitive. *)
+
+CoInductive semantics_equiv {i} : semantics i -> semantics i -> Prop :=
+| semantics_equiv_rec
+    (sem sem' : semantics i)
+    (step_equiv : forall {a} (e : i a),
+        interp_out_equiv (run_effect sem e) (run_effect sem' e))       (* (1) *)
+  : semantics_equiv sem sem'
+
+(** Two interpretation output are said equivalent when (1) they carry the same
+    result, and they provide equivalent semantics to use afterwards. *)
+
+with interp_out_equiv {i} : forall {a : Type}, interp_out i a -> interp_out i a -> Prop :=
+| step_equiv {a}
+    (o o' : interp_out i a)
+    (res_eq : interp_result o = interp_result o')                      (* (1) *)
+    (next_equiv : semantics_equiv (interp_next o) (interp_next o'))    (* (2) *)
+  : interp_out_equiv o o'.
+
+(** We prove [semantics_equiv] is an equivalence, that is the relation is (1)
+    reflexive, (2) symmetric, and (3) transitive. *)
+
+#[program]
+Instance semantics_equiv_Equivalence (i : interface) : Equivalence (@semantics_equiv i).
+
+Obligation 1.
+  cofix semantics_equiv_refl.
+  intros sem.
+  constructor.
+  intros a e.
+  constructor; [ reflexivity |].
+  apply semantics_equiv_refl.
+Qed.
+
+Obligation 2.
+  cofix semantics_equiv_sym.
+  intros sem sem' equiv.
+  destruct equiv as [sem sem' step].
+  constructor.
+  intros a e.
+  specialize step with a e.
+  destruct step.
+  constructor.
+  + now symmetry.
+  + now apply semantics_equiv_sym.
+Qed.
+
+Obligation 3.
+  cofix semantics_equiv_trans.
+  intros sem sem' sem'' equiv equiv'.
+  destruct equiv as [sem sem' equ].
+  destruct equiv' as [sem' sem'' equ'].
+  constructor; intros a e.
+  specialize equ with a e.
+  specialize equ' with a e.
+  inversion equ; ssubst.
+  inversion equ'; ssubst.
+  constructor.
+  + now transitivity (eval_effect sem' e).
+  + eapply semantics_equiv_trans; [ apply next_equiv | apply next_equiv0 ].
+Qed.
+
+(** We use [semantics_equiv] as the [Equality] relation for [semantics]. *)
+
+#[program]
+Instance semantics_Equality (i : interface) : Equality (semantics i).
+
+#[global]
+Opaque semantics_Equality.
+
+(** We proceed similarly with [interp_out_equiv]: we first prove it is an
+    equivalence, then we use this relation as the [Equality] relation for
+    [interp_out]. *)
+
+#[program]
+Instance interp_out_Equivalence (i : interface) (a : Type)
+  : Equivalence (@interp_out_equiv i a).
+
+Obligation 1.
+  intros [x sem].
+  constructor; reflexivity.
+Qed.
+
+Obligation 2.
+  intros o o' equ.
+  inversion equ; ssubst.
+  now constructor.
+Qed.
+
+Obligation 3.
+  intros o o' o'' equ equ'.
+  inversion equ; ssubst.
+  inversion equ'; ssubst.
+  constructor.
+  + now transitivity (interp_result o').
+  + now transitivity (interp_next o').
+Qed.
+
+#[program]
+Instance interp_out_Equality (i : interface) (a : Type) : Equality (interp_out i a).
+
+#[global]
+Opaque interp_out_Equality.
+
+(** Since [interp_out_equiv] and [semantics_equiv] are two equivalence, we can
+    use them with the [rewrite] tactics, as long as we provide valid [Proper]
+    instances.  We proceed accordingly in FreeSpec.Core, as systematically as
+    possible. *)
+
+#[program]
+Instance mk_out_Proper (i : interface) (a : Type)
+  : Proper (eq ==> 'equal ==> 'equal) (@mk_out i a).
+
+Next Obligation.
+  add_morphism_tactic.
+  intros x sem sem' equ.
+  constructor.
+  + reflexivity.
+  + apply equ.
+Qed.
+
+#[program]
+Instance run_effect_Proper (i : interface) (a : Type)
+  : Proper ('equal ==> eq ==> 'equal) (@run_effect i a).
+
+Next Obligation.
+  add_morphism_tactic.
+  intros sem sem' equ p.
+  inversion equ; ssubst.
+  apply step_equiv0.
+Qed.
+
+#[program]
+Instance interp_result_Proper (i : interface) (a : Type)
+  : Proper ('equal ==> eq) (@interp_result i a).
+
+Next Obligation.
+  add_morphism_tactic.
+  intros o o' equ.
+  now inversion equ; ssubst.
+Qed.
+
+#[program]
+Instance interp_next_Proper (i : interface) (a : Type)
+  : Proper ('equal ==> 'equal) (@interp_next i a).
+
+Next Obligation.
+  add_morphism_tactic.
+  intros o o' equ.
+  now inversion equ; ssubst.
+Qed.
+
+#[program]
+Instance eval_effect_Proper (i : interface) (a : Type)
+  : Proper ('equal ==> eq ==> eq) (@eval_effect i a).
+
+Next Obligation.
+  add_morphism_tactic.
+  intros o o' equ e.
+  unfold eval_effect.
+  now rewrite equ.
+Qed.
+
+#[program]
+Instance exec_effect_Proper (i : interface) (a : Type)
+  : Proper ('equal ==> eq ==> 'equal) (@exec_effect i a).
+
+Next Obligation.
+  add_morphism_tactic.
+  intros o o' equ e.
+  unfold exec_effect.
+  now rewrite equ.
+Qed.
+
+Lemma semantics_equiv_interp_next_effect {i a}
+  (sem sem' : semantics i) (equ : sem == sem') (e : i a)
+  : interp_next (run_effect sem e) == interp_next (run_effect sem' e).
+Proof.
+  inversion equ; ssubst.
+  specialize step_equiv0 with a e.
+  inversion step_equiv0; ssubst.
+  apply next_equiv.
+Qed.
+
+Hint Resolve semantics_equiv_interp_next_effect : freespec.
+
+Lemma semantics_equiv_exec_effect {i a}
+  (sem sem' : semantics i) (equ : sem == sem') (e : i a)
+  : exec_effect sem e == exec_effect sem' e.
+Proof.
+  unfold exec_effect.
+  auto with freespec.
+Qed.
+
+Hint Resolve semantics_equiv_exec_effect : freespec.
+
+#[program]
+Instance semplus_Proper (i j : interface)
+  : Proper ('equal ==> 'equal ==> 'equal) (@semplus i j).
+
+Next Obligation.
+  add_morphism_tactic.
+  cofix semplus_Proper.
+  intros semi semi' equi semj semj' equj.
+  constructor.
+  intros a e.
+  destruct e; constructor; cbn.
+  + now rewrite equi.
+  + apply semplus_Proper; auto with freespec.
+  + now rewrite equj.
+  + apply semplus_Proper; auto with freespec.
+Qed.
+
+(** * Impure Computations *)
+
+(** We introduce the [impure] monad to describe impure computations, that is
+    computations which uses primitives from certain interfaces.
+
+    ** Definition
+
+    The [impure] monad is an inductive datatype with two parameters: the
+    interface [i] to be used, and the type [a] of the result of the computation.
+    The fact that [impure] is inductive rather than co-inductive means it is not
+    possible to describte infinite computations.  This also means it is possible
+    to interpret impure computation within Coq, providing an operational
+    semantics for [i]. *)
+
+Inductive impure (i : interface) (a : Type) : Type :=
+| local (x : a) : impure i a
+| request_then {b} (e : i b) (f : b -> impure i a) : impure i a.
+
+Arguments local [i a] (x).
+Arguments request_then [i a b] (e f).
+
+(** ** Equivalence *)
+
+Inductive impure_equiv {i a} : impure i a -> impure i a -> Prop  :=
+| local_equiv (x : a) : impure_equiv (local x) (local x)
+| request_equiv {b} (e : i b) (f g : b -> impure i a)
+    (equ : forall (x : b), impure_equiv (f x) (g x))
+  : impure_equiv (request_then e f) (request_then e g).
+
+#[program]
+Instance impure_equiv_Equivalence (i : interface) (a : Type)
+  : Equivalence (@impure_equiv i a).
+
+Next Obligation.
+  intros p.
+  induction p; constructor.
+  intros x.
+  apply H.
+Qed.
+
+Next Obligation.
+  intros p q equ.
+  induction equ; constructor.
+  intros x.
+  apply H.
+Qed.
+
+Next Obligation.
+  intros p q r pq qr.
+  revert p r pq qr.
+  induction q; intros p r pq qr.
+  + inversion pq; ssubst; inversion qr; ssubst.
+    constructor.
+  + inversion pq; ssubst; inversion qr; ssubst.
+    constructor.
+    intros x.
+    now apply H with (b := x).
+Qed.
+
+#[program]
+Instance impure_Equality (i : interface) (a : Type) : Equality (impure i a).
+
+#[global]
+Opaque impure_Equality.
+
+(** ** Monad Instances *)
+
+(* FIXME[0]: This works because coq-prelude provides a default [Equality]
+   instance for any type is [eq].  Since [b] is universally quantified, there is
+   no specific instance to pick expect this one, and therefore the instance of
+   Equality for [a -> b] is [forall x, f x = g x], which is exactly what we
+   need. *)
+#[program]
+Instance request_then_Proper (i : interface) (a b : Type)
+  : Proper (eq ==> 'equal ==> 'equal) (@request_then i a b).
+
+Next Obligation.
+  add_morphism_tactic.
+  intros x f g equ.
+  now constructor.
+Qed.
+
+Fixpoint impure_bind {i a b} (p : impure i a) (f : a -> impure i b) : impure i b :=
+  match p with
+  | local x => f x
+  | request_then e g => request_then e (fun x => impure_bind (g x) f)
+  end.
+
+#[program]
+Instance impure_bind_Proper_1 (i : interface) (a b : Type)
+  : Proper (eq ==> 'equal ==> 'equal) (@impure_bind i a b).
+
+Next Obligation.
+  add_morphism_tactic.
+  intros p f g equf.
+  induction p.
+  + apply equf.
+  + constructor.
+    intros sem.
+    apply H.
+Qed.
+
+#[program]
+Instance impure_bind_Proper_2 (i : interface) (a b : Type)
+  : Proper ('equal ==> eq ==> 'equal) (@impure_bind i a b).
+
+Next Obligation.
+  add_morphism_tactic.
+  intros p q equp f.
+  induction equp.
+  + reflexivity.
+  + cbn.
+    constructor.
+    apply H.
+Qed.
+
+Ltac change_request_then :=
+  match goal with
+  | |- request_then ?e ?f == request_then ?e ?g =>
+    let R := fresh "R" in
+    assert (R: f == g); [ intros ?x | rewrite R; clear R ]
+  end.
+
+Ltac change_impure_bind :=
+  match goal with
+  | |- impure_bind ?e ?f == impure_bind ?e ?g =>
+    let R := fresh "R" in
+    assert (R: f == g); [ intros ?x | now rewrite R ]
+  end.
+
+Lemma impure_bind_local {i a} (p : impure i a) : impure_bind p (@local i a) == p.
+Proof.
+  induction p.
+  + reflexivity.
+  + cbn.
+    change_request_then; [| reflexivity ].
+    now rewrite H.
+Qed.
+
+Lemma impure_bind_assoc {i a b c}
+  (p : impure i a) (f : a -> impure i b) (g : b -> impure i c)
+  : impure_bind (impure_bind p f) g == impure_bind p (fun x => impure_bind (f x) g).
+Proof.
+  induction p; [reflexivity |].
+  cbn.
+  change_request_then; [| reflexivity ].
+  now rewrite H.
+Qed.
+
+(* see FIXME[0] *)
+Definition impure_map {i a b} (f : a -> b) (p : impure i a) : impure i b :=
+  impure_bind p (fun x => local (f x)).
+
+#[program]
+Instance impure_map_Proper (i : interface) (a b : Type)
+  : Proper ('equal ==> 'equal ==> 'equal) (@impure_map i a b).
+
+Next Obligation.
+  add_morphism_tactic.
+  intros f g equf p q equp.
+  unfold impure_map.
+  rewrite equp.
+  change_impure_bind.
+  now rewrite equf.
+Qed.
+
+#[program]
+Instance impure_Functor (i : interface) : Functor (impure i) :=
+  { map := @impure_map i
+  }.
+
+Next Obligation.
+  unfold impure_map.
+  now rewrite impure_bind_local.
+Defined.
+
+Next Obligation.
+  unfold compose.
+  unfold impure_map.
+  now rewrite impure_bind_assoc.
+Defined.
+
+Definition impure_pure {i a} : a -> impure i a :=
+  @local i a.
+
+Definition impure_apply {i a b} (p : impure i (a -> b)) (q : impure i a) : impure i b :=
+  impure_bind p (fun f => map f q).
+
+#[program]
+Instance impure_apply_Proper (i : interface) (a b : Type)
+  : Proper ('equal ==> 'equal ==> 'equal) (@impure_apply i a b).
+
+Next Obligation.
+  add_morphism_tactic.
+  intros p q equ1 r s equ2.
+  unfold impure_apply.
+  rewrite equ1.
+  change_impure_bind.
+  cbn.
+  now rewrite equ2.
+Qed.
+
+#[program, polymorphic]
+Instance impure_Applicative (i : interface) : Applicative (impure i) :=
+  { pure := @impure_pure i
+  ; apply := @impure_apply i
+  }.
+
+Next Obligation.
+  unfold impure_apply, impure_pure, impure_bind.
+  now rewrite functor_identity.
+Defined.
+
+Next Obligation.
+  unfold impure_apply, impure_pure; cbn.
+  unfold impure_map.
+  repeat rewrite impure_bind_assoc.
+  change_impure_bind; cbn.
+  repeat rewrite impure_bind_assoc.
+  change_impure_bind; cbn.
+  repeat rewrite impure_bind_assoc.
+  now change_impure_bind.
+Defined.
+
+Next Obligation.
+  reflexivity.
+Qed.
+
+Next Obligation.
+  reflexivity.
+Qed.
+
+Next Obligation.
+  reflexivity.
+Qed.
+
+#[program]
+Instance impure_Monad (i : interface) : Monad (impure i) :=
+  { bind := @impure_bind i
+  }.
+
+Next Obligation.
+  reflexivity.
+Defined.
+
+Next Obligation.
+  now rewrite impure_bind_local.
+Defined.
+
+Next Obligation.
+  now rewrite impure_bind_assoc.
+Defined.
+
+Next Obligation.
+  now change_impure_bind.
+Defined.
+
+Next Obligation.
+  reflexivity.
+Defined.
+
+(** ** Defining Impure Computations *)
+
+(** FreeSpec users shall not use the [impure] monad constructors directly.  The
+    [pure] function from the [Applicative] typeclass allows for defining pure
+    computations which do not depend on any impure primitive.  The [bind]
+    function from the [Monad] typeclass allows for seamlessly combine impure
+    computations together.
+
+    To complete these two monadic operation, we introduce the [request]
+    function, whose purpose is to define an impure computation that uses a given
+    primitive [e] from an interface [i], and returns its result.  [request] does
+    not parameterize the [impure] monad with [i] directly, but rather with a
+    generic interface [ix].  [ix] is constrained with the [Provide] notation, so
+    that it has to provide at least [i]'s primitives.  *)
+
+Definition request {ix i} `{ix :| i} {a : Type} (e : i a) : impure ix a :=
+  request_then (lift_eff e) (fun x => local x).
+
+(** The ~coq-prelude~ provides notations (inspired by the do notation of
+    Haskell) to write monadic functions more easily.  These notations live
+    inside the [monad_scope] scope. *)
+
+Bind Scope monad_scope with impure.
+
+(** ** Interpreting Impure Computations *)
+
+Fixpoint run_impure {i a} (sem : semantics i) (p : impure i a) : interp_out i a :=
+  match p with
+  | local x =>
+    mk_out x sem
+  | request_then e f =>
+    let s := run_effect sem e in
+    run_impure (interp_next s) (f (interp_result s))
+  end.
+
+Definition eval_impure {i a} (sem : semantics i) (p : impure i a) : a :=
+  interp_result (run_impure sem p).
+
+Definition exec_impure {i a} (sem : semantics i) (p : impure i a) : semantics i :=
+  interp_next (run_impure sem p).
+
+Lemma run_impure_request_then_equ {i a b} (sem : semantics i)
+  (e : i a) (f : a -> impure i b)
+  : run_impure sem (request_then e f) = run_impure (exec_effect sem e) (f (eval_effect sem e)).
+Proof eq_refl.
+
+Hint Rewrite @run_impure_request_then_equ : freespec.
+
+Lemma semantics_equiv_interp_next_impure {i a}
+  (sem sem' : semantics i) (equ : sem == sem') (p : impure i a)
+  : interp_next (run_impure sem p) == interp_next (run_impure sem' p).
+Proof.
+  revert sem sem' equ.
+  induction p; intros sem sem' equ.
+  + apply equ.
+  + cbn.
+    unfold exec_impure.
+    cbn.
+    rewrite equ at 2.
+    apply H.
+    auto with freespec.
+Qed.
+
+Hint Resolve semantics_equiv_interp_next_impure : freespec.
+
+Lemma semantics_equiv_exec_impure {i a}
+  (sem sem' : semantics i) (equ : sem == sem') (p : impure i a)
+  : exec_impure sem p == exec_impure sem' p.
+Proof.
+  unfold exec_impure.
+  auto with freespec.
+Qed.
+
+Hint Resolve semantics_equiv_exec_impure : freespec.
+
+#[program]
+Instance run_impure_Proper_1 (i : interface) (a : Type)
+  : Proper ('equal ==> eq ==> 'equal) (@run_impure i a).
+
+Next Obligation.
+  add_morphism_tactic.
+  intros sem sem' equ p.
+  revert sem sem' equ.
+  induction p; intros sem sem' equ.
+  + cbn.
+    now rewrite equ.
+  + cbn.
+    rewrite equ at 2.
+    auto with freespec.
+Qed.
+
+#[program]
+Instance run_impure_Proper_2 (i : interface) (a : Type)
+  : Proper (eq ==> 'equal ==> 'equal) (@run_impure i a).
+
+Next Obligation.
+  add_morphism_tactic.
+  intros sem p q equ.
+  revert sem.
+  induction equ; intros sem.
+  + reflexivity.
+  + apply H.
+Qed.
+
+#[program]
+Instance eval_impure_Proper (i : interface) (a : Type)
+  : Proper ('equal ==> 'equal ==> eq) (@eval_impure i a).
+
+Next Obligation.
+  add_morphism_tactic.
+  intros sem sem' equ1 p q equ2.
+  unfold eval_impure.
+  now rewrite equ1, equ2.
+Qed.
+
+#[program]
+Instance exec_impure_Proper (i : interface) (a : Type)
+  : Proper ('equal ==> 'equal ==> 'equal) (@exec_impure i a).
+
+Next Obligation.
+  add_morphism_tactic.
+  intros sem sem' equ1 p q equ2.
+  unfold exec_impure.
+  now rewrite equ1, equ2.
+Qed.
+
+Lemma run_impure_equiv {i a} (p q : impure i a) (equ : p == q) (sem : semantics i)
+  : run_impure sem p == run_impure sem q.
+Proof.
+  now rewrite equ.
+Qed.
+
+Hint Resolve run_impure_equiv : freespec.
+
+Lemma run_impure_exec_impure_equiv {i a}
+  (sem sem' : semantics i) (p q : impure i a) (equ : run_impure sem p == run_impure sem' q)
+  : exec_impure sem p == exec_impure sem' q.
+Proof.
+  now inversion equ; ssubst.
+Qed.
+
+Hint Resolve run_impure_exec_impure_equiv : freespec.
+
+Lemma run_impure_eval_impure_equiv {i a}
+  (sem sem' : semantics i) (p q : impure i a) (equ : run_impure sem p == run_impure sem' q)
+  : eval_impure sem p = eval_impure sem' q.
+Proof.
+  now inversion equ; ssubst.
+Qed.
+
+Hint Resolve run_impure_eval_impure_equiv : freespec.
+
+Lemma exec_impure_equiv {i a} (p q : impure i a) (equ : p == q) (sem : semantics i)
+  : exec_impure sem p == exec_impure sem q.
+Proof.
+  now rewrite equ.
+Qed.
+
+Hint Resolve run_impure_equiv : freespec.
+
+Lemma impure_bind_equation {i a b}
+  (p : impure i a) (f : a -> impure i b) (sem : semantics i)
+  : run_impure sem (impure_bind p f)
+    == run_impure (exec_impure sem p) (f (eval_impure sem p)).
+Proof.
+  revert sem.
+  induction p; intros sem.
+  + reflexivity.
+  + cbn.
+    apply H.
+Qed.
+
+(** * Component
+
+    In FreeSpec, we call a component an entity which exposes an interface [i],
+    and uses primitives of an interface [j] to compute the result of primitives
+    of [i].  Besides, a component is likely to carry its own internal state (of
+    type [s]).
+
+<<
+                               c : component i j s
+                           i +---------------------+      j
+                           | |                     |      |
+                   +------>| |       st : s        |----->|
+                           | |                     |      |
+                             +---------------------+
+>>
+
+    Thus, a component [c : component i j s] is a polymorphic function which,
+    given a primitive of [i], and the current state of the component, maps
+    impure computations which return the result of the primitive and the new
+    state of the component.  We use the State monad [state_t] to handle the
+    internal state of the component more easily.  We could have use the [STORE
+    s] interface discussed previously, but we believe using [state_t] simplifies
+    the reasoning process of FreeSpec. *)
+
+Definition component (i j : interface) (s : Type) : Type :=
+  forall (a : Type), i a -> state_t s (impure j) a.
+
+
+(** The similarity between FreeSpec components and operational semantics may be
+    confusing at first.  The main difference between the two concepts is simple:
+    operational semantics are self-contained terms which can, alone, be used to
+    interpret impure computations of a given interface.  Components, on the
+    other hand, are not self-contained.  Without an intial state [init : s] and
+    an operational semantics for [j], we cannot use a component [c : component i
+    j s] to interpret an impure computation using [i].
+
+    Given an initial state and and initial semantics for [j], we can however
+    derive an operational semantics for [i] from a component [c]. *)
+
+CoFixpoint derive_semantics {i j s} (c : component i j s) (st : s) (sem : semantics j) :=
+  mk_semantics (fun (a : Type) (e : i a) =>
+                  let out := run_impure sem (c a e st) in
+                  let res := interp_result out in
+                  let sem' := interp_next out in
+                  mk_out (fst res) (derive_semantics c (snd res) sem')).
+
+(** So, [⊕] on the onde hand allows for composing operational semantics
+    horizontally, and [derive_semantics] allows for composing components
+    vertically.  Using these two operators, we can model a complete system in a
+    modular manner, by defining each of its component independently, then
+    composing them together with [⊕] and [derive_semantics]. *)
+
+Definition bootstrap {i s} (c : component i ⋄ s) (st : s) :=
+  derive_semantics c st semempty.
